coq/Common/FMapExt.v
@@ -1,0 +1,123 @@
+Require Import Coq.ZArith.BinInt.
+Require Import Coq.FSets.FMapAVL.
+From Coq.Structures Require Import OrderedType OrderedTypeEx.
+
+From ExtLib.Data Require Import List.
+From ExtLib.Structures Require Import Monad Monads Traversable.
+
+From Coq.Lists Require Import List. (* after exltlib *)
+
+Require Import Utils.
+
+Local Open Scope type_scope.
+Local Open Scope list_scope.
+Local Open Scope monad_scope.
+
+Import MonadNotation.
+
+Require Import Coq.FSets.FMapFacts.
+
+(* Ordered type with additional operations *)
+Module Type OrderedTypeExt.
+  Include UsualOrderedType.
+
+  Parameter with_offset: t -> Z -> t.
+  Parameter of_nat: nat -> t.
+  Parameter of_Z: Z -> t.
+End OrderedTypeExt.
+
+(* FMap with additional operatons and properties. *)
+Module Type FMapExt
+  (OT:OrderedTypeExt).
+
+  Module Import M := FMapAVL.Make(OT).
+  Module Import P := FMapFacts.WProperties_fun(OT)(M).
+  Module Import F := FMapFacts.WFacts_fun(OT)(M).
+
+  Fixpoint map_range_init {T} (a0:M.key) (n:nat) (step:Z) (v:T) (m:M.t T) : M.t T
+    :=
+    match n with
+    | O => m
+    | S n =>
+        let m := map_range_init a0 n step v m in
+        M.add (OT.with_offset a0 (Z.mul (Z.of_nat n) step)) v m
+    end.
+
+  Definition map_update_element
+    {A:Type}
+    (key: M.key)
+    (v: A)
+    (m: M.t A)
+    : (M.t A)
+    :=
+    M.add key v (M.remove key m).
+
+  (** [update key f m] returns a map containing the same bindings as
+  [m], except for the binding of [key]. Depending on the value of [y]
+  where [y] is [f (find_opt key m)], the binding of [key] is added,
+  removed or updated. If [y] is [None], the binding is removed if it
+  exists; otherwise, if [y] is [Some z] then key is associated to [z]
+  in the resulting map. *)
+  Definition map_update
+    {A:Type}
+    (key: M.key)
+    (f: option A -> option A)
+    (m: M.t A)
+    : (M.t A)
+    :=
+    let y := f (M.find key m) in
+    let m' := M.remove key m in (* could be optimized, as removal may be unecessary in some cases *)
+    match y with
+    | None => m'
+    | Some z => M.add key z m'
+    end.
+
+  Definition map_sequence
+    {A: Type}
+    {m: Type -> Type}
+    {M: Monad m}
+    (mv: M.t (m A)): m (M.t A)
+    :=
+    let (kl,vl) := List.split (M.elements mv) in
+    vl' <- sequence (F:=m) (T:=list) vl ;;
+    ret (of_list (combine kl vl')).
+
+  (** Adds elements of given [list] to a [map] starting at [addr]. *)
+  Definition map_add_list_at
+    {T:Type}
+    (map: M.t T)
+    (list: list T)
+    (addr: M.key)
+    : M.t T
+    :=
+    let ilist :=
+      Utils.mapi
+        (fun (i: nat) (v: T) =>
+           ((OT.with_offset addr (Z.of_nat i)), v)
+        )
+        list in
+    List.fold_left (fun acc '(k, v) =>  M.add k v acc) ilist map.
+
+  (* Monadic mapi *)
+  Definition map_mmapi
+    {A B : Type}
+    {m : Type -> Type}
+    {M : Monad m}
+    (f : M.key -> A -> m B) (zm: M.t A)
+    : m (M.t B)
+    :=
+    map_sequence (M.mapi f zm).
+
+  Definition map_find_first {A:Type} (f:M.key -> A -> bool) (m:M.t A): option (M.key * A)
+    :=
+    M.fold (fun k v (acc:option (M.key * A)) =>
+              match acc with
+              | None => if f k v
+                       then Some (k, v)
+                       else None
+              | Some _ => acc
+              end)
+      m None.
+
+End FMapExt.
+
